Everything having to do with freshness or strict extension of states should be dead

coq/LLVMGen/Correctness_Invariants.v
@@ -31,7 +31,6 @@ Section WF_IRState.
     forall v n, nth_error σ n ≡ Some v ->
            exists id, (nth_error Γ n ≡ Some (id, getWFType id (DSHType_of_DSHVal v))).
 
-
   Definition WF_IRState (σ : evalContext) (s : IRState) : Prop :=
     evalContext_typechecks σ (Γ s).
 
@@ -132,7 +131,6 @@ Ltac abs_by_WF :=
       now (let EQ := fresh in destruct h as [EQ | [EQ | [? EQ]]]; inv EQ)
     end
   end.
-
 
 Ltac try_abs :=
   try (abs_by_WF ||
@@ -405,6 +403,7 @@ Section SimulationRelations.
       The main invariant carried around combine the two properties defined:
       1. the memories satisfy the invariant;
       2. the [IRState] is well formed;
+      3. 
    *)
   Record state_invariant (σ : evalContext) (s : IRState) (memH : memoryH) (configV : config_cfg) : Prop :=
     {
@@ -1076,87 +1075,10 @@ Section SimulationRelations.
 
 End SimulationRelations.
 
-Section Ext_Local.
-
-  (** When compiling expressions, we need to carry on the invariant that
-      the meaning of the generated expression will be stable by execution of the
-      intermediate code corresponding to the evaluation of the second operand.
-      To this end, we rely on the fact that this code does not alter the configuration
-      except to extend it with fresh bindings.
-   *)
-  Definition ext_local {R S}: config_helix -> config_cfg -> Rel_cfg_T R S :=
-    fun mh '(mi,(li,gi)) '(mh',_) '(m,(l,(g,_))) => mh ≡ mh' /\ mi ≡ m /\ gi ≡ g /\ li ⊑ l.
-
-  Definition sub_local_no_aliasing (σ : evalContext) (s : IRState) (ρ1 ρ2 : local_env) (g : global_env) :=
-    ρ1 ⊑ ρ2 /\ no_llvm_ptr_aliasing σ s ρ2 g.
-
-  Definition ext_local_no_aliasing {R S}
-             (σ : evalContext) (s  : IRState) :
-    config_helix -> config_cfg -> Rel_cfg_T R S
-    := fun mh '(mi,(li,gi)) '(mh',_) '(m,(l,(g,_))) =>
-         mh ≡ mh' /\ mi ≡ m /\ gi ≡ g /\ sub_local_no_aliasing σ s li l g.
-
-  Lemma in_local_or_global_scalar_ext_local :
-    forall ρ1 ρ2 g m x dv τ,
-      in_local_or_global_scalar ρ1 g m x dv τ ->
-      ρ1 ⊑ ρ2 ->
-      in_local_or_global_scalar ρ2 g m x dv τ.
-  Proof.
-    unfold in_local_or_global_scalar; intros ? ? ? ? [] ? ? IN MONO; auto.
-    apply MONO; auto.
-  Qed.
-
-  Lemma in_local_or_global_addr_ext_local :
-    forall ρ1 ρ2 g x ptr,
-      in_local_or_global_addr ρ1 g x ptr ->
-      ρ1 ⊑ ρ2 ->
-      in_local_or_global_addr ρ2 g x ptr.
-  Proof.
-    unfold in_local_or_global_addr; intros ρ1 ρ2 g [] ptr IN MONO; auto.
-    apply MONO; auto.
-  Qed.
-
-  Lemma no_llvm_ptr_aliasing_ext_local :
-    forall σ s ρ1 ρ2 g,
-      no_llvm_ptr_aliasing σ s ρ1 g ->
-      sub_local_no_aliasing σ s ρ1 ρ2 g ->
-      no_llvm_ptr_aliasing σ s ρ2 g.
-  Proof.
-    intros σ s ρ1 ρ2 g ALIAS [EXT EXT_ALIAS].
-    eauto.
-  Qed.
-
-
-  Lemma memory_invariant_ext_local :
-    forall σ s memH memV ρ1 ρ2 g,
-      memory_invariant σ s memH (memV, (ρ1, g)) ->
-      ρ1 ⊑ ρ2 ->
-      memory_invariant σ s memH (memV, (ρ2, g)).
-  Proof.
-    intros * MEM_INV EXT_LOCAL.
-    red; intros * NTH NTH'.
-    specialize (MEM_INV _ _ _ _ NTH NTH').
-    destruct v; eauto.
-    eapply in_local_or_global_scalar_ext_local; eauto.
-    eapply in_local_or_global_scalar_ext_local; eauto.
-    repeat destruct MEM_INV as (? & MEM_INV).
-    do 3 eexists; splits; eauto.
-    eapply in_local_or_global_addr_ext_local; eauto.
-  Qed.
-
-End Ext_Local.
-
 Lemma state_invariant_WF_IRState :
   forall σ s memH st, state_invariant σ s memH st -> WF_IRState σ s.
 Proof.
   intros ? ? ? (? & ? & ?) INV; inv INV; auto.
-Qed.
-
-Lemma ext_local_refl:
-  forall {R S} memH memV l g n v,
-    @ext_local R S memH (mk_config_cfg memV l g) (memH, n) (memV, (l, (g, v))).
-Proof.
-  intros; repeat split; reflexivity.
 Qed.
 
 Lemma in_local_or_global_scalar_same_global : forall l g l' m id dv τ,
@@ -1197,32 +1119,6 @@ Proof.
   rewrite remove_neq_alist; auto; try typeclasses eauto; intros ->; auto.
 Qed.
 
-Lemma fresh_no_lu :
-  forall s s' id l g m x dv τ,
-    incLocal s ≡ inr (s', id) ->
-    incLocal_fresh l s ->
-    in_local_or_global_scalar l g m x dv τ ->
-    x <> ID_Local id.
-Proof.
-  intros * INC FRESH IN abs; subst.
-  apply FRESH in INC.
-  unfold alist_fresh in *.
-  cbn in *; rewrite INC in IN; inv IN.
-Qed.
-
-Lemma fresh_no_lu_addr :
-  forall s s' id l g x ptr,
-    incLocal s ≡ inr (s', id) ->
-    incLocal_fresh l s ->
-    in_local_or_global_addr l g x ptr ->
-    x <> ID_Local id.
-Proof.
-  intros * INC FRESH IN abs; subst.
-  apply FRESH in INC.
-  unfold alist_fresh in *.
-  cbn in *; rewrite INC in IN; inv IN.
-Qed.
-
 Lemma append_factor_left : forall s s1 s2,
     s @@ s1 ≡ s @@ s2 ->
     s1 ≡ s2.
@@ -1231,14 +1127,6 @@ Proof.
   apply IH.
   inv EQ; auto.
 Qed.
-
-Lemma ext_local_subalist : forall {R S} memH memV l1 g vH vV l2,
-    l1 ⊑ l2 ->
-    @ext_local R S memH (mk_config_cfg memV l1 g) (memH, vH) (memV, (l2, (g, vV))).
-Proof.
-  intros * SUB; cbn; splits; auto.
-Qed.
-
 
 Lemma state_invariant_incLocal :
   forall σ s s' k memH stV,
@@ -1350,18 +1238,6 @@ Proof.
   auto.
 Qed.
 
-Lemma state_invariant_sub_local_no_aliasing_refl :
-  forall l g s mh mv σ,
-    state_invariant σ s mh (mv, (l, g)) ->
-    sub_local_no_aliasing σ s l l g.
-Proof.
-  intros l g s mh mv σ SINV.
-  destruct SINV. cbn in *.
-  split; [reflexivity | eauto].
-Qed.
-
-Hint Resolve state_invariant_sub_local_no_aliasing_refl: core.
-
 Lemma unsigned_is_zero: forall a, Int64.unsigned a ≡ Int64.unsigned Int64.zero ->
                                   a = Int64.zero.
 Proof.
@@ -1384,68 +1260,6 @@ Proof.
   intros id p0 p' H0 H1.
   specialize (PTR p0).
   contradiction.
-Qed.
-
-(* Lemma sub_local_no_aliasing_add_non_ptr : *)
-(*   forall σ s id v l g, *)
-(*     alist_fresh id l -> *)
-(*     no_llvm_ptr_aliasing σ s l g -> *)
-(*     sub_local_no_aliasing σ s l (alist_add id v l) g. *)
-(* Proof. *)
-(*   intros σ s id v l g FRESH ALIAS. *)
-(*   unfold sub_local_no_aliasing. *)
-(*   split. *)
-
-(*   - apply sub_alist_add; auto. *)
-(*   - epose proof (no_llvm_ptr_aliasing_not_in_gamma' _ ALIAS FRESH). *)
-(*     unfold no_llvm_ptr_aliasing in ALIAS. *)
-(*     intros id0 id' ptr ptr' n1 n2 ptrh1 ptrh2 τ τ' sz1 sz2 H0 H1 H2 H3 H4. *)
-(*     unfold no_llvm_ptr_aliasing in H. *)
-(*     eapply H; [apply H0 | apply H1 | apply H2 | apply H3 | apply H4 ]. *)
-(* Qed. *)
-
-Lemma sub_local_no_aliasing_transitive :
-  forall σ s l0 l1 l2 g,
-    sub_local_no_aliasing σ s l0 l1 g ->
-    sub_local_no_aliasing σ s l1 l2 g ->
-    sub_local_no_aliasing σ s l0 l2 g.
-Proof.
-  intros σ s l0 l1 l2 g [L0L1 ALIAS1] [L1L2 ALIAS2].
-  split; eauto.
-  etransitivity; eauto.
-Qed.
-
-Lemma sub_local_no_aliasing_add_non_ptr' :
-  forall σ s id v l l' g,
-    alist_fresh id l ->
-    ~ in_Gamma σ s id ->
-    WF_IRState σ s ->
-    no_llvm_ptr_aliasing σ s l g ->
-    sub_local_no_aliasing σ s l' l g ->
-    sub_local_no_aliasing σ s l' (alist_add id v l) g.
-Proof.
-  intros σ s id v l l' g FRESH NGAMMA WF ALIAS [L'L ALIAS'].
-  unfold sub_local_no_aliasing.
-  split.
-
-  - rewrite L'L. apply alist_le_add; auto.
-  - epose proof (no_llvm_ptr_aliasing_not_in_gamma _ ALIAS).
-    unfold no_llvm_ptr_aliasing in *.
-    intros * H0 H1 H2 H3 H4 H5 H6.
-    eapply H;     
-      [eauto | eauto | apply H0 | apply H1 | apply H2 | apply H3 | apply H4 | apply H5 | apply H6].
-Qed.
-
-Lemma sub_local_no_aliasing_Γ :
-  forall σ s1 s2 l1 l2 g,
-    sub_local_no_aliasing σ s1 l1 l2 g ->
-    Γ s2 ≡ Γ s1 ->
-    sub_local_no_aliasing σ s2 l1 l2 g.
-Proof.
-  intros σ s1 s2 l1 l2 g [L1L2 SUB] GAMMA.
-  unfold sub_local_no_aliasing, no_llvm_ptr_aliasing in *.
-  rewrite GAMMA.
-  auto.
 Qed.
 
 Lemma no_llvm_ptr_aliasing_gamma :
@@ -1472,13 +1286,6 @@ Proof.
   auto.
 Qed.
 
-
-(* TODO: might not need this anymore *)
-(* Ltac solve_no_local_global_alias := *)
-(*   solve *)
-(*     [ let H := fresh in *)
-(*       apply no_local_global_alias_non_pointer; intros ? H; discriminate H ]. *)
-
 Ltac solve_alist_in := first [apply In_add_eq | idtac].
 Ltac solve_lu :=
   (try now eauto);
@@ -1492,46 +1299,6 @@ Ltac solve_lu :=
   | _ => solve_alist_in
   end.
 
-Ltac solve_state_invariant :=
-  cbn; try eassumption;
-  match goal with
-  | |- state_invariant _ _ _ (_, (alist_add _ _ _, _)) =>
-    eapply state_invariant_add_fresh; [now eauto | solve_alist_fresh | (eassumption || solve_state_invariant) | solve_fresh]
-  | |- state_invariant _ _ _ _ =>
-    solve [eauto with SolveStateInv]
-  end.
-
-Hint Extern 2 (state_invariant _ _ _ _) => eapply state_invariant_incBlockNamed; [eassumption | solve_state_invariant] : SolveStateInv.
-Hint Extern 2 (state_invariant _ _ _ _) => eapply state_invariant_incLocal; [eassumption | solve_state_invariant] : SolveStateInv.
-Hint Extern 2 (state_invariant _ _ _ _) => eapply state_invariant_incVoid; [eassumption | solve_state_invariant] : SolveStateInv.
-
-Ltac solve_sub_local_no_aliasing_gamma :=
-  match goal with
-  | H: incLocal ?s1 ≡ inr (?s2, _) |- sub_local_no_aliasing ?σ ?s2 ?l1 ?l2 ?g
-    => let GAMMA := fresh "GAMMA"
-       in assert (Γ s2 ≡ Γ s1) as GAMMA by eauto with helix_context;
-          eapply sub_local_no_aliasing_Γ;
-          eauto;
-          clear GAMMA
-
-  | H: genNExpr _ ?s1 ≡ inr (?s2, _) |- sub_local_no_aliasing ?σ ?s2 ?l1 ?l2 ?g
-    => let GAMMA := fresh "GAMMA"
-       in assert (Γ s2 ≡ Γ s1) as GAMMA by eauto with helix_context;
-          eapply sub_local_no_aliasing_Γ;
-          eauto;
-          clear GAMMA
-
-  | H: genNExpr _ ?s1 ≡ inr (?s2, _),
-       SUB: sub_local_no_aliasing ?σ ?s2 ?l1 ?l2 ?g |- _
-    => let GAMMA := fresh "GAMMA" in
-       let SUB2  := fresh "SUB" in
-       assert (Γ s1 ≡ Γ s2) as GAMMA by eauto with helix_context;
-       epose proof (sub_local_no_aliasing_Γ _ SUB GAMMA);
-       clear SUB;
-       eauto
-  end.
-
-
 Ltac solve_in_gamma :=
   match goal with
   | GAM : nth_error (Γ ?s) ?n ≡ Some (ID_Local ?id, _),
@@ -1544,7 +1311,6 @@ Ltac solve_in_gamma :=
 Ltac solve_lid_bound_between :=
   eapply lid_bound_between_shrink; [eapply lid_bound_between_incLocal | | ]; eauto; solve_local_count.
 
-
 Ltac solve_not_in_gamma :=
   first [ now eauto
         |
@@ -1556,27 +1322,11 @@ Ltac solve_not_in_gamma :=
     | solve [eapply not_in_Gamma_Gamma_eq; [eassumption | solve_not_in_gamma]]
     ].
 
-Ltac solve_sub_local_no_aliasing :=
-  first [ solve [eapply state_invariant_sub_local_no_aliasing_refl; solve_state_invariant]
-        | solve_sub_local_no_aliasing_gamma; solve_sub_local_no_aliasing
-        | eapply sub_local_no_aliasing_add_non_ptr';
-          [ solve_alist_fresh
-          | solve_not_in_gamma
-          | eauto
-          | eapply state_invariant_no_llvm_ptr_aliasing; solve_state_invariant
-          | solve_sub_local_no_aliasing
-          ]
-        | solve [eapply sub_local_no_aliasing_transitive; eauto]].
-Definition state_invariant_pre σ s1 s2 := (state_invariant σ s1 ⩕ fresh_pre s1 s2).
-Definition state_invariant_post σ s1 s2 l := (state_invariant σ s2 ⩕ fresh_post s1 s2 l).
-
 Hint Resolve state_invariant_memory_invariant : core.
 Hint Resolve memory_invariant_GLU memory_invariant_LLU memory_invariant_LLU_AExpr memory_invariant_GLU_AExpr : core.
 
 Hint Resolve is_pure_refl: core.
-Hint Resolve state_invariant_memory_invariant state_invariant_WF_IRState ext_local_refl: core.
 Hint Resolve local_scope_modif_refl: core.
-Hint Resolve memory_invariant_ext_local: core.
 
 (* TODO: Move this, and remove Transparent / Opaque *)
 Lemma incLocal_unfold :
